coq/Recursion.v
@@ -1,0 +1,300 @@
+(** *Total functional programming *)
+
+From TypingFlags Require Import Loader.
+From Equations Require Import Equations.
+Require Import Coq.Program.Equality.
+Require Import MPRICoq.Monad.
+Require Import MPRICoq.Indexed.
+
+(** **First order unification *)
+
+Module UnifSpec.
+  Import Maybe.
+
+  (** ***Specification: terms *)
+  Definition Var := nat.
+  Inductive Term : Type :=
+  | var (i : Var) : Term
+  | leaf : Term
+  | fork (s t : Term) : Term.
+
+  Fixpoint sub (ρ : Var -> Term) (t : Term) : Term :=
+    match t with
+    | var i => ρ i
+    | leaf => leaf
+    | fork s t => fork (sub ρ s) (sub ρ t)
+    end.
+
+  Definition comp_sub (ρ1 ρ2 : Var -> Term) (t : Var) : Term :=
+    sub ρ1 (ρ2 t).
+  Notation "ρ1 ∘K ρ2" := (comp_sub ρ1 ρ2) (at level 30).
+
+  (** ***Specification: occur-check *)
+  Fixpoint diff (x : Var) (y : Var) : Maybe Var :=
+    match x, y with
+    | O, O => None
+    | O, S y => ret y
+    | S x, O => ret O
+    | S x, S y => (diff x y) >>= fun y' => ret (S y')
+    end.
+  Notation "x △ y" := (diff x y) (at level 30).
+
+  Fixpoint check (i : Var) (t : Term) : Maybe Term :=
+    match t with
+    | var j => i △ j >>= fun z => ret (var z)
+    | leaf => ret leaf
+    | fork f s => check i f >>= fun r1 => check i s >>= fun r2 => ret (fork r1 r2)
+    end.
+
+  (** ***Specification: substitution *)
+  Inductive Subst : Type :=
+  | id : Subst
+  | subst (σ : Subst)(i : Var)(t : Term) : Subst.
+  Notation "σ :: [ i ↦ t ]" := (subst σ i t) (at level 30).
+
+  Definition substitute (t : Term) (i : Var) : Var -> Term :=
+    fun j => match i △ j with
+          | None => t
+          | Some j' => var j'
+          end.
+
+  Reserved Notation "⟦ ρ ⟧".
+  Fixpoint apply_subst (ρ : Subst) : Var -> Term :=
+    match ρ with
+    | id => fun x => var x
+    | ρ::[i ↦ t] => fun x => (⟦ρ⟧ ∘K (substitute t i)) x
+    end
+  where "⟦ ρ ⟧" := (apply_subst ρ).
+
+  (** ***Specification: most-general unifier *)
+  Definition flex_flex (x y : Var) : Subst :=
+    match x △ y with
+    | Some y' => id::[x ↦ var y']
+    | None => id
+    end.
+
+  Definition flex_rigid x t := check x t >>= fun t' => ret (id::[x ↦ t']).
+
+  (** We will assume thag the program actually terminates, but the Coq's
+      termination checker wont be able to prove it; we switch the checker off
+      for now *)
+  Unset Guard Checking.
+  Fixpoint amgu (t1 : Term) (t2 : Term) (σ : Subst) {struct t1} : Maybe Subst :=
+    match t1, t2, σ with
+    (* Conflicts: *)
+    | leaf, (fork _ _), _ => None
+    | (fork _ _), leaf, _ => None
+    (* Matches: *)
+    | leaf, leaf, acc => ret acc
+    | (fork s1 t1), (fork s2 t2), acc => amgu s1 s2 acc >>= amgu t1 t2
+    (* Variables flex-flex: *)
+    | (var x), (var y), id => ret (flex_flex x y)
+    (* Variables flex-rigid: *)
+    | (var x), t, id => flex_rigid x t
+    | t, (var x), id => flex_rigid x t
+    | t1, t2, σ::[z ↦ r] => amgu (sub (substitute r z) t1)
+                        (sub (substitute r z) t2) σ >>= fun σ => ret (σ::[z ↦ r])
+    end.
+  Set Guard Checking.
+
+  Definition mgu (s t : Term) : Maybe Subst := amgu s t id.
+
+  Example test1 : mgu (fork (var 0) leaf) (fork (fork leaf leaf) (var 1))
+                  = Some (id::[0 ↦ leaf]::[0 ↦ fork leaf leaf]).
+  Proof. reflexivity. Qed.
+
+  Example test2 : mgu (fork (var 0) leaf) (fork (fork leaf leaf) (var 3))
+                  = Some (id::[2 ↦ leaf]::[0 ↦ (fork leaf leaf)]).
+  Proof. reflexivity. Qed.
+
+  Example test3 : mgu (var 0) (fork leaf (var 0))
+                  = None.
+  Proof. reflexivity. Qed.
+
+  Example test4 : mgu (fork (var 0) leaf) (fork (fork leaf leaf) (var 0))
+                  = None.
+  Proof. reflexivity. Qed.
+
+  Example test5 : mgu (fork (var 0) (var 1))
+                      (fork (fork leaf (var 1)) (fork leaf leaf))
+                  = Some (id::[0 ↦ (fork leaf leaf)]::[0 ↦ (fork leaf (var 0))]).
+  Proof. reflexivity. Qed.
+End UnifSpec.
+
+Module UnifStruct.
+  Import Maybe.
+  Import NormalForms.Fin.
+
+  (** ***Structurally: terms *)
+
+  (** We now stratify the set of variables, ie. `Var n` contains `n`
+      distinct variables: *)
+  Definition Var : nat -> Type := fin.
+
+  (** We can thus represent terms with (at most) ``n`` variables: *)
+  Inductive Term (n : nat) : Type :=
+  | var (i : Var n) : Term n
+  | leaf : Term n
+  | fork (s t : Term n) : Term n.
+  Arguments var {_}. Arguments leaf {_}. Arguments fork {_}.
+
+  Fixpoint sub {m n} (ρ : Var m -> Term n) (t : Term m) : Term n :=
+    match t with
+    | var i => ρ i
+    | leaf => leaf
+    | fork s t => fork (sub ρ s) (sub ρ t)
+    end.
+
+  Definition comp_sub {m n l}
+             (ρ1 : Var m -> Term n) (ρ2 : Var l -> Term m) (t : Var l) : Term n :=
+    sub ρ1 (ρ2 t).
+  Notation "ρ1 ∘K ρ2" := (comp_sub ρ1 ρ2) (at level 30).
+
+  Fixpoint ren {m n} (ρ : Var m -> Var n) (t : Term m) : Term n :=
+    match t with
+    | var v => var (ρ v)
+    | leaf => leaf
+    | fork s t => fork (ren ρ s) (ren ρ t)
+    end.
+
+  Definition subst_eq {m n} (f g : Var m -> Term n) : Prop :=
+    forall x, f x = g x.
+  Notation "f ≗ g" := (subst_eq f g) (at level 80).
+
+  Fixpoint diff {n} (x : Var (S n)) (y : Var (S n)) : Maybe (Var n).
+  Proof.
+    inversion x; inversion y; subst.
+    - exact None.
+    - exact (ret i).
+    - destruct n.
+      + inversion i.
+      + exact (ret zero).
+    - destruct n.
+      + inversion i.
+      + exact (diff _ i i0 >>= fun y' => ret (suc y')).
+  Defined.
+  Notation "x △ y" := (diff x y) (at level 30).
+
+  Fact diff_zero_l : forall {n} (i : Var n), zero △ (suc i) = Some i.
+  Proof.
+    intros n i.
+    destruct i; reflexivity.
+  Qed.
+
+  (* Equations inj {n} : Var (S n) -> Var n -> Var (S n) := *)
+  (*   { inj zero y := suc y; *)
+  (*     inj (suc x) zero := zero; *)
+  (*     inj (suc x) (suc y) := suc (inj x y) *)
+  (*   }. *)
+  Fixpoint inj {n} (x : Var (S n)) (y : Var n) : Var (S n).
+  Proof.
+    inversion x as [?|? x']; subst; clear x.
+    - exact (suc y).
+    - inversion y as [?|? y']; subst; clear y.
+      + exact zero.
+      + exact (suc (inj _ x' y')).
+  Defined.
+  Notation "inj[ x ]" := (inj x).
+
+  Lemma lemma_inj1 : forall {n : nat} (x : Var (S n)) y z, inj[x] y = inj[x] z -> y = z.
+  Proof.
+    fix inj1 2.
+    intros n x y z Heq.
+    dependent destruction x; simpl in Heq; unfold eq_rect_r, eq_rect, eq_sym in *.
+    - apply fin_eq_suc in Heq. assumption.
+    - dependent destruction y; simpl; dependent destruction z; simpl in *;
+        try congruence.
+      + apply fin_eq_suc in Heq.
+        apply inj1 in Heq. rewrite Heq. reflexivity.
+  Qed.
+
+  Lemma lemma_inj2 : forall {n : nat} (x : Var (S n)) y, inj[x] y <> x.
+  Proof.
+    fix inj2 2.
+    intros n x y.
+    dependent destruction x; simpl; unfold eq_rect_r, eq_rect, eq_sym.
+    - congruence.
+    - dependent destruction y.
+      + try congruence.
+      + intro contra. apply fin_eq_suc in contra.
+        congruence.
+  Qed.
+
+  Lemma lemma_inj_diff : forall {n : nat} (x y : Var (S n)) (r : Maybe (Var n)),
+      x △ y = r -> (x = y /\ r = None) \/ (exists y', y = inj[x] y' /\ r = Some y').
+  Proof.
+    fix inj_diff 2.
+    intros n x y r Hdiff.
+    destruct n; dependent destruction x; dependent destruction y; simpl in *;
+      unfold eq_rect_r, eq_rect, eq_sym in *;
+      try (now (left;auto));
+      try (now (inversion x));
+      try (now (inversion y)).
+    - right. exists y; auto.
+    - right. exists zero; auto.
+    - destruct (inj_diff _ x y (x △ y)); auto.
+      + left. destruct H as [H1 H2].
+        rewrite H1. rewrite H2 in Hdiff. auto.
+      + right. destruct H as [y' [Hy1 Hy2]].
+        rewrite Hy2 in Hdiff.
+        exists (suc y'). rewrite Hy1. auto.
+  Qed.
+
+  Inductive inj_View {n} (i : Var (S n)) : (Var (S n)) -> Type :=
+  | just (k : Var n) : inj_View i (inj[i] k)
+  | eq : inj_View i i.
+
+  (** ***Structurally: occur-check *)
+  Fixpoint check {n} (i : Var (S n)) (t : Term (S n)) : Maybe (Term n) :=
+    match t with
+    | var j => i △ j >>= fun k => ret (var k)
+    | leaf => ret leaf
+    | fork f s => check i f >>= fun r1 => check i s >>= fun r2 => ret (fork r1 r2)
+    end.
+
+  Lemma lemma_check : forall {n : nat} x t {t'},
+      @check n x t = Some t' -> ren (inj[x]) t' = t.
+  Proof.
+    fix lemma_check 3.
+    intros n x t t' Hcheck.
+    destruct t; simpl in *.
+    - destruct (x △ i) eqn:Hdiff; try congruence.
+      inversion Hcheck; subst; clear Hcheck.
+      dependent destruction x; simpl;
+        unfold eq_rect_r, eq_rect, eq_sym.
+      + admit.
+      + admit.
+    - inversion Hcheck; subst.
+      dependent destruction x; simpl;
+        unfold eq_rect_r, eq_rect, eq_sym; reflexivity.
+    - destruct (check x t1) eqn:Hcheck1; try congruence.
+      destruct (check x t2) eqn:Hcheck2; try congruence.
+      apply lemma_check in Hcheck1; apply lemma_check in Hcheck2; simpl in *.
+      dependent destruction x; simpl in *;
+        unfold eq_rect_r, eq_rect, eq_sym in *; simpl in *;
+          inversion Hcheck; subst; reflexivity.
+  Admitted.
+
+  (** ***Structurally: single term substitution *)
+  Definition substitute {n} (t : Term n) (i : Var (S n)) : Var (S n) -> Term n :=
+    fun j => match i △ j with
+          | None => t
+          | Some j' => var j'
+          end.
+
+  Lemma lemma_for_inj : forall {n} (t : Term n) x,
+      (fun v => substitute t x (inj[x] v)) ≗ var.
+  Proof.
+    intros n t x.
+    unfold subst_eq. intros v.
+    dependent destruction x; simpl in *;
+      unfold eq_rect_r, eq_rect, eq_sym in *.
+    - unfold substitute. destruct t; simpl; rewrite diff_zero_l; reflexivity.
+    - dependent destruction v; simpl in *.
+      + reflexivity.
+      + unfold substitute; simpl.
+        unfold eq_rect_r, eq_rect, eq_sym.
+  Admitted.
+
+  (* TODO *)
+End UnifStruct.
